\documentclass{article}
\usepackage{amsmath}
\usepackage{amssymb}

\begin{document}

\begin{equation}
    \text{Please type me! The quick brown fox jumps over the lazy dog.}
\end{equation}

\begin{equation}
    e^{i\pi} + 1 = 0
\end{equation}

\begin{equation}
    e^{i\theta} = \cos\theta + i\sin\theta
\end{equation}

\begin{equation}
    G_{\mu\nu} + \Lambda g_{\mu\nu} = \frac{8\pi G}{c^4} T_{\mu\nu}
\end{equation}

\begin{equation}
    x = \frac{-b \pm \sqrt{b^2 - 4ac}}{2a}
\end{equation}

\begin{equation}
    \vec{L} = \vec{r} \times \vec{p}
\end{equation}

\begin{equation}
    \sqrt[3]{2}
\end{equation}

\begin{equation}
    (x + y)^n = \sum_{r=0}^n \binom{n}{r} x^r y^{n-r}
\end{equation}

\begin{equation}
    \sqrt{\frac{a_1^2 + \cdots + a_n^2}{n}} \geq \frac{a_1 + \cdots + a_n}{n} \geq \sqrt[n]{a_1 \cdots a_n} \geq \frac{n}{\frac{1}{a_1} + \cdots + \frac{1}{a_n}}
\end{equation}

\begin{equation}
    | \langle x, y \rangle |^2 \leq \langle x, x \rangle \cdot \langle y, y \rangle
\end{equation}

\begin{equation}
\begin{aligned}
    \text{A1: } &\varphi \rightarrow (\psi \rightarrow \varphi) \\
    \text{A2: } &(\varphi \rightarrow (\psi \rightarrow \theta)) \rightarrow ((\varphi \rightarrow \psi) \rightarrow (\varphi \rightarrow \theta)) \\
    \text{A3: } &(\neg \varphi \rightarrow \neg \psi) \rightarrow (\psi \rightarrow \varphi)
\end{aligned}
\end{equation}

\end{document}